# baseURI http://adp.athlinks.com/2017/01/rdf-schema#

@prefix athlinks: <http://adp.athlinks.com/2017/01/rdf-schema#> .
@prefix rdf: <http://www.w3.org/1999/02/22-rdf-syntax-ns#> .
@prefix owl: <http://www.w3.org/2002/07/owl#> .
@prefix xsd: <http://www.w3.org/2001/XMLSchema#> .
@prefix rdfs: <http://www.w3.org/2000/01/rdf-schema#> .
@prefix schema: <http://schema.org/> .

<http://adp.athlinks.com/2017/01/rdf-schema> a owl:Ontology ;
  owl:imports <http://topbraid.org/schema/> ;
  rdfs:label "The Athlinks Schema vocabulary".

### CLASSES
athlinks:TimingInterval
  a rdfs:Class ;
  rdfs:comment "A measured distance over all or part of an athletic event course." ;
  rdfs:label "Timing interval" ;
  rdfs:subClassOf schema:Place .
  #members:
  #athlinks:defaultPace;
  #athlinks:distanceFromStart;
  #athlinks:distance;
  #schema:fromLocation;
  #schema:toLocation;

athlinks:TimingPoint a rdfs:Class;
  rdfs:subClassOf schema:Place;
  rdfs:label "Timing point";
  rdfs:comment "A point located within a timing interval at which sensors are deployed to capture tag reads of passing athletes.".

athlinks:TagRead a rdfs:Class;
  rdfs:label "RFID tag read";
  rdfs:comment "The representation of a raw reading of an RFID tag." .
  #members:
  #athlinks:timingDevice;
  #schema:agent;
  #schema:location;
  #athlinks:rawTime;
  #athlinks:adjustedTime.

athlinks:IntervalResult a rdfs:Class;
  rdfs:label "Interval Result";
  rdfs:comment "The duration calculated for an interval by an actor.";
  rdfs:subClassOf schema:MoveAction .
  #members:
  #athlinks:beginTagRead;
  #athlinks:endTagRead;
  #athlinks:bib;
  #schema:duration;
  #athlinks:timingInterval;
  #athlinks:ranking;
  #athlinks:chipTime ;
  #athlinks:clockTime .

athlinks:BracketRanking a rdfs:Class;
  rdfs:label "Bracket Ranking";
  rdfs:comment "A raking of an Interval Result when ranked within a Bracket." .
  #members:
  #athlinks:bracket;
  #athlinks:intervalResult;
  #athlinks:timingInterval;
  #athlinks:rank;
  #athlinks:agePercentage.

athlinks:Bracket a rdfs:Class.

athlinks:AthleticRace
  a owl:Class ;
  rdfs:comment "An athletic race, a distinct course." ;
  rdfs:label "Athletic Race" ;
  rdfs:subClassOf schema:SportsEvent .
  #members:
  #athlinks:raceType ;
  #ageReferenceDate.

athlinks:AthleticEvent
  a owl:Class ;
  rdfs:comment "An Athletic Event, a group of Athletic Races that are all part of the same event." ;
  rdfs:label "Athletic Race" ;
  rdfs:subClassOf schema:SportsEvent .

athlinks:AthleticEventGroup
  a owl:Class ;
  rdfs:comment "An Athletic Event Group.  This can be any sort of grouping of events...manually grouped, recurring, etc..." ;
  rdfs:label "Athletic Event Group" ;
  rdfs:subClassOf schema:SportsEvent .
  #members:
  #athlinks:subEventGroup;
  #athlinks:visibility;
  #athlinks:recurrence;
  #athlinks:scoring.

athlinks:ActivityFeature
  a owl:Class ;
  rdfs:subClassOf schema:QualitativeValue ;
  rdfs:comment "Flag describing an activity"@en ;
  rdfs:label "ActivityFeature"@en .

## INSTANCES
athlinks:RunUpTo5k a athlinks:ActivityFeature ;
    rdfs:comment "Instance of a flag indicating activity in a running event up to 5k in distance" ;
    rdfs:label "Run up to 5k" .
athlinks:Run5kTo15k a athlinks:ActivityFeature ;
    rdfs:comment "Instance of a flag indicating activity in a running event from 5k to 15k in distance" ;
    rdfs:label "Run 5k to 15k" .
athlinks:Run15kToHalfMarathon a athlinks:ActivityFeature ;
    rdfs:comment "Instance of a flag indicating activity in a running event from 15k to Half Marathon in distance" ;
    rdfs:label "Run 15k to Half Marathon" .
athlinks:RunHalfToFullMarathon a athlinks:ActivityFeature ;
    rdfs:comment "Instance of a flag indicating activity in a running event from Half Marathon to Full Marathon in distance" ;
    rdfs:label "Run Half Marathon to Marathon" .
athlinks:RunMarathon a athlinks:ActivityFeature ;
    rdfs:comment "Instance of a flag indicating activity in a Marathon running event" ;
    rdfs:label "Run Marathon" .
athlinks:RunUltra a athlinks:ActivityFeature ;
    rdfs:comment "Instance of a flag indicating activity in a Ultra-marathon running event" ;
    rdfs:label "Run Ultra" .
athlinks:MultisportSprint a athlinks:ActivityFeature ;
    rdfs:comment "Instance of a flag indicating activity in a Triathlon Sprint athletic event" ;
    rdfs:label "Sprint Triathlon" .
athlinks:MultisportOlympic a athlinks:ActivityFeature ;
    rdfs:comment "Instance of a flag indicating activity in a Triathlon Olympic athletic event" ;
    rdfs:label "Olympic Triathlon" .
athlinks:MultisportHalfIronman a athlinks:ActivityFeature ;
    rdfs:comment "Instance of a flag indicating activity in a Half Ironman athletic event" ;
    rdfs:label "Half Ironman" .
athlinks:MultisportIronMan a athlinks:ActivityFeature ;
    rdfs:comment "Instance of a flag indicating activity in an Ironman athletic event" ;
    rdfs:label "Ironman" .
athlinks:Aquathlon a athlinks:ActivityFeature ;
    rdfs:comment "Instance of a flag indicating activity in an Aquathlon athletic event" ;
    rdfs:label "Aquathlon" .
athlinks:Aquabike a athlinks:ActivityFeature ;
    rdfs:comment "Instance of a flag indicating activity in an Aquabike athletic event" ;
    rdfs:label "Aquabike" .
athlinks:Duathlon a athlinks:ActivityFeature ;
    rdfs:comment "Instance of a flag indicating activity in a Duathlon athletic event" ;
    rdfs:label "Duathlon" .
athlinks:Swim a athlinks:ActivityFeature ;
    rdfs:comment "Instance of a flag indicating activity in a Swimming athletic event" ;
    rdfs:label "Swim" .
athlinks:MountainBike a athlinks:ActivityFeature ;
    rdfs:comment "Instance of a flag indicating activity in a Mountain Bike athletic event" ;
    rdfs:label "Mountain Bike" .
athlinks:Cycling a athlinks:ActivityFeature ;
    rdfs:comment "Instance of a flag indicating activity in a Cycling athletic event" ;
    rdfs:label "Cycling" .
athlinks:Snow a athlinks:ActivityFeature ;
    rdfs:comment "Instance of a flag indicating activity in a Snowshow Running athletic event" ;
    rdfs:label "Snowshow Running" .
athlinks:Adventure a athlinks:ActivityFeature ;
    rdfs:comment "Instance of a flag indicating activity in an Adventure athletic event" ;
    rdfs:label "Adventure" .
athlinks:Obstacle a athlinks:ActivityFeature ;
    rdfs:comment "Instance of a flag indicating activity in an Obstacle Course athletic event" ;
    rdfs:label "Obstacle" .
athlinks:Other a athlinks:ActivityFeature ;
    rdfs:comment "Instance of a flag indicating activity in an athletic event not described" ;
    rdfs:label "Other" .

## PROPERTIES

athlinks:rank a owl:DataTypeProperty;
  rdfs:domain athlinks:BracketRanking;
  rdfs:range schema:Integer.

athlinks:timingInterval a owl:ObjectProperty;
  rdfs:domain athlinks:IntervalResult;
  rdfs:label "The Interval component of the course";
  schema:rangeIncludes schema:ExerciseAction .

athlinks:bracket a owl:ObjectProperty;
  rdfs:domain athlinks:BracketRanking;
  rdfs:range athlinks:Bracket.

athlinks:endTagRead a owl:ObjectProperty;
  rdfs:domain athlinks:IntervalResult;
  rdfs:range athlinks:TagRead.

athlinks:beginTagRead a owl:ObjectProperty;
  rdfs:domain athlinks:IntervalResult;
  rdfs:range athlinks:TagRead.

athlinks:timingDevice a owl:ObjectProperty;
  rdfs:domain athlinks:TagRead;
  rdfs:range schema:Thing.

athlinks:rawTime a owl:DataTypeProperty;
  rdfs:domain athlinks:TagRead;
  rdfs:range schema:DateTime.

athlinks:adjustedTime a owl:DataTypeProperty;
  rdfs:domain athlinks:TagRead;
  rdfs:range schema:DateTime.

athlinks:ranking a owl:ObjectProperty;
  rdfs:domain athlinks:IntervalResult;
  rdfs:range athlinks:BracketRanking.

athlinks:defaultPace
  a owl:ObjectProperty ;
  rdfs:domain athlinks:TimingInterval ;
  rdfs:range schema:QuantitativeValue .

athlinks:distanceFromStart
  a owl:ObjectProperty ;
  rdfs:domain athlinks:TimingInterval ;
  rdfs:range schema:QuantitativeValue .

athlinks:distance
  a owl:ObjectProperty ;
  rdfs:range schema:QuantitativeValue .

athlinks:raceType
  a owl:DataTypeProperty;
  rdfs:range [ a xsd:string ;
                owl:oneOf ("triathlon" "5k" "10k" "marathon" "other")
              ] .
athlinks:raceActivityType a owl:ObjectProperty ;
  rdfs:domain athlinks:AthleticRace ;
  rdfs:range [
    a athlinks:ActivityFeature ;
    owl:oneOf (athlinks:RunUpTo5k athlinks:Run5kTo15k athlinks:Run15kToHalfMarathon athlinks:RunHalfToFullMarathon athlinks:RunMarathon athlinks:RunUltra athlinks:MultisportSprint athlinks:MultisportOlympic athlinks:MultisportHalfIronman athlinks:MultisportIronMan athlinks:Aquathlon athlinks:Aquabike athlinks:Duathlon athlinks:Swim athlinks:MountainBike athlinks:Cycling athlinks:Snow athlinks:Adventure athlinks:Obstacle athlinks:Other)
  ] ;
  rdfs:comment "An indication of the type of ActivityFeature that a race is."@en ;
  rdfs:label "race activity type"@en .

athlinks:bib
  a owl:DataTypeProperty;
  rdfs:range xsd:string .

athlinks:pace
  a owl:DataTypeProperty ;
  rdfs:range schema:QuantitativeValue .

athlinks:clockTime
  a owl:DataTypeProperty ;
  rdfs:domain athlinks:IntervalResult;
  rdfs:range schema:Duration .

athlinks:chipTime
  a owl:DataTypeProperty ;
  rdfs:domain athlinks:IntervalResult;
  rdfs:range schema:Duration .

athlinks:agePercentage
  a owl:DataTypeProperty ;
  rdfs:domain athlinks:IntervalResult;
  rdfs:range xsd:decimal .

athlinks:ageReferenceDate a owl:DataTypeProperty;
  rdfs:label "Age Reference Date";
  rdfs:comment "When event has a minimum age, this is the date by which they must be that age." ;
  rdfs:domain athlinks:AthleticRace ;
  rdfs:range schema:Date .

athlinks:subEventGroup
  a owl:ObjectProperty;
  rdfs:comment "A list of AthleticEventGroups" ;
  rdfs:domain athlinks:AthleticEventGroup ;
  rdfs:range athlinks:AthleticEventGroup .

athlinks:visibility
  a owl:DataTypeProperty ;
  rdfs:comment "Denotes who has access to see an object";
  rdfs:label "Visibility Access" ;
  rdfs:domain athlinks:AthleticEventGroup ;
  rdfs:range [ a xsd:string ;
                owl:oneOf ("Private" "Friends" "Invite" "Public")
              ] .

athlinks:recurrence
  a owl:DataTypeProperty ;
  rdfs:label "Schedule Recurrance";
  rdfs:comment "The default recurrence of a certain scheduling item";
  rdfs:domain athlinks:AthleticEventGroup ;
  rdfs:range [ a xsd:string ;
                owl:oneOf ("Monthly" "Yearly" "None")
              ] .

athlinks:scoring
  a owl:ObjectProperty ;
  rdfs:comment "The scoring used on an AthleticEventGroup" ;
  rdfs:domain athlinks:AthleticEventGroup .

athlinks:directions a owl:ObjectProperty ;
  rdfs:comment "Directions to an event or race." ;
  rdfs:domain schema:Event ;
  rdfs:label "Directions" ;
  rdfs:range schema:Text.

athlinks:participatedIn a owl:ObjectProperty ;
  rdfs:domain schema:Person ;
  rdfs:range [
    a athlinks:ActivityFeature ;
    owl:oneOf (athlinks:RunUpTo5k athlinks:Run5kTo15k athlinks:Run15kToHalfMarathon athlinks:RunHalfToFullMarathon athlinks:RunMarathon athlinks:RunUltra athlinks:MultisportSprint athlinks:MultisportOlympic athlinks:MultisportHalfIronman athlinks:MultisportIronMan athlinks:Aquathlon athlinks:Aquabike athlinks:Duathlon athlinks:Swim athlinks:MountainBike athlinks:Cycling athlinks:Snow athlinks:Adventure athlinks:Obstacle athlinks:Other)
  ] ;
  rdfs:comment "An indication of a person participating in an ActivityFeature."@en ;
  rdfs:label "participated in"@en .

athlinks:numberOfRaces a owl:DataTypeProperty ;
  rdfs:comment "Number of races completed by an athlete." ;
  rdfs:label "Number of races" ;
  rdfs:domain schema:Person ;
  rdfs:range xsd:unsignedInt .

athlinks:GenderNotSpecified a schema:GenderType ;
  rdfs:comment "Used when a person does not want to specify their gender" ;
  rdfs:label "Athlinks Gender Not Specified" .
